IrisCore/BaseLogicDeepExperimental.thy
@@ -1,0 +1,209 @@
+theory BaseLogicDeepExperimental
+imports CoreStructures Namespace "../HeapLang/PrimitiveLaws" Frac DerivedConstructions
+  "../SpanningTree/SpanningTreeCameras" "../HeapLang/State"
+begin
+
+text \<open> An experimental approach to a deep embedding of the Iris base/core logic.\<close>
+
+text \<open>Deep embedding of camera objects\<close>
+datatype 'a cmra_term = ConstC 'a | Core \<open>'a cmra_term\<close> | Op \<open>'a cmra_term\<close> \<open>'a cmra_term\<close>
+
+text \<open>Deep embedding of step-index predicates about camera objects\<close>
+datatype 'a cmra_atom = 
+  Own \<open>'a cmra_term\<close> \<comment> \<open>Holds for camera objects which include the given partial resource\<close>
+| Valid \<open>'a cmra_term\<close>
+
+type_synonym 'a res = "(graphUR auth \<times> markingUR auth \<times> 'a \<times> heap_lang_heap)"
+
+text \<open>Predicate connectives\<close>
+datatype iprop = 
+  Atom \<open>inv res cmra_atom\<close> \<comment> \<open>An atomic predicate about camera resources\<close>
+  \<comment> \<open>Standard separation logic connectives\<close>
+| Sep iprop iprop \<comment> \<open>Separating conjunction\<close>
+| Wand iprop iprop \<comment> \<open>Wand combinator, i.e. resource specific implication\<close>
+| Pure bool \<comment> \<open>Wrapper for pure Isabelle/HOL propositions\<close>
+  \<comment> \<open>Iris specific modalities\<close>
+| Persistent iprop \<comment> \<open>Predicate holds for core of the camera argument\<close>
+| Plain iprop \<comment> \<open>Predicate holds for unit camera object\<close>
+| Later iprop \<comment> \<open>Increases step index by one (also holds for n=0)\<close>
+| BUpd iprop \<comment> \<open>Predicate holds after one frame-preserving update\<close>
+  \<comment> \<open>Standard logic connectives\<close>
+| Impl iprop iprop
+| Conj iprop iprop
+| Disj iprop iprop
+  \<comment> \<open>Extensions that can not be defined without unfortunate complexity\<close>
+| InvP namespace iprop
+and inv = Inv \<open>(name\<rightharpoonup> iprop later ag) auth \<times> name dset \<times> name dfset\<close>
+
+instance inv :: ucamera sorry
+instance iprop :: ofe sorry
+
+type_synonym atom = "inv res cmra_atom"
+
+primrec cmra_eval :: "'a::ucamera cmra_term \<Rightarrow> 'a" where
+  "cmra_eval (ConstC a) = a"
+| "cmra_eval (Core a) = core (cmra_eval a)"
+| "cmra_eval (Op a b) = (cmra_eval a) \<cdot> (cmra_eval b)"
+
+type_synonym upred = "inv res \<Rightarrow> nat \<Rightarrow> bool"
+
+primrec atom_sem :: "atom \<Rightarrow> upred" where
+  "atom_sem (Own a) b n = n_incl n (cmra_eval a) b"
+| "atom_sem (Valid a) _ n = n_valid (cmra_eval a) n"
+
+fun pred_sem :: "iprop \<Rightarrow> upred" and inv_sem :: "inv \<Rightarrow> upred"
+where
+  "pred_sem (Atom a) = (\<lambda>b n. atom_sem a b n)"
+| "pred_sem (Sep P Q) = (\<lambda>a n. (\<exists>b1 b2. n_equiv n a (b1 \<cdot> b2) \<and> pred_sem P b1 n \<and> pred_sem Q b2 n))"
+| "pred_sem (Wand P Q) = (\<lambda>a n.
+  (\<forall>m b. m\<le>n \<and> n_valid (a \<cdot> b) m \<longrightarrow> pred_sem P b m \<longrightarrow> pred_sem Q (a \<cdot> b) m))"
+| "pred_sem (Pure b) = (\<lambda>_ _.  b)"
+| "pred_sem (Persistent P) = (\<lambda>a n. pred_sem P (core a) n)"
+| "pred_sem (Plain P) = (\<lambda>_ n. pred_sem P \<epsilon> n)"
+| "pred_sem (Later P) = (\<lambda>a n. (n=0 \<or> pred_sem P a (n-1)))"
+| "pred_sem (BUpd P) = (\<lambda>a n.
+  (\<forall>m a'. m\<le>n \<and> n_valid (a \<cdot> a') m \<longrightarrow> (\<exists>b. n_valid (b \<cdot> a') m \<and> pred_sem P b m)))"
+| "pred_sem (Impl P Q) = (\<lambda>a n.
+  (\<forall>m b. m\<le>n \<and> incl a b \<and> n_valid b m \<longrightarrow> pred_sem P b m \<longrightarrow> pred_sem Q b m))"
+| "pred_sem (Conj P Q) = (\<lambda>a n. (pred_sem P a n \<and> pred_sem Q a n))"
+| "pred_sem (Disj P Q) = (\<lambda>a n. (pred_sem P a n \<or> pred_sem Q a n))"
+| "pred_sem (InvP N P) = (\<lambda>a n.
+  (\<exists>\<iota>. \<iota> \<in> names N \<and> atom_sem (Own (ConstC (\<epsilon>,\<epsilon>,Inv (fragm [\<iota>\<mapsto>to_ag (Next P)],\<epsilon>,\<epsilon>),\<epsilon>))) a n))"
+| "inv_sem (Inv _) _ _ = True"
+  
+definition uniform :: "upred \<Rightarrow> bool" where
+  "uniform f \<longleftrightarrow> (\<forall>n m x y. f x n \<longrightarrow> n_incl m x y \<longrightarrow> m\<le>n \<longrightarrow> f y m)"
+
+lemma upred_weaken: "\<lbrakk>n_equiv n x y; m\<le>n;uniform f; f x n\<rbrakk> \<Longrightarrow> f y m"
+  using total_n_inclI uniform_def by fast
+
+lemma upred_weaken_simple: "\<lbrakk>uniform f; f x n; m\<le>n\<rbrakk> \<Longrightarrow> f x m"
+  using ofe_refl upred_weaken by blast
+  
+lemma atom_sem_uniform: "uniform (atom_sem a)"
+proof (induct a)
+  case (Own x)
+  then show ?case unfolding uniform_def n_incl_def atom_sem.simps
+  using camera_assoc op_equiv_subst by (metis (no_types, lifting))
+next
+  case (Valid x)
+  then show ?case by (simp add: uniform_def)
+qed
+
+lemma pred_sem_uniform: "uniform (pred_sem P)"
+proof (induct P rule: iprop.induct[of "\<lambda>_. True"])
+  case (Atom x)
+  then show ?case by (simp) (rule atom_sem_uniform)
+next
+  case (Sep P Q)
+  then have Q: "\<And>n m x y. \<lbrakk>(pred_sem Q) x n; n_incl m x y; m\<le>n\<rbrakk> \<Longrightarrow> (pred_sem Q) y m"
+    by (auto simp: uniform_def)
+  {
+    fix n m x y
+    assume assms: "pred_sem (Sep P Q) x n" "n_incl m x y" "m\<le>n"
+    then obtain b1 b2 where bs: "n_equiv n x (b1 \<cdot> b2)" "(pred_sem P) b1 n" "(pred_sem Q) b2 n"
+      by auto
+    from assms(2) obtain z where z: "n_equiv m y (x \<cdot> z)" by (auto simp: n_incl_def)
+    from op_equiv_subst[OF this bs(1) assms(3)] camera_assoc have "n_equiv m y (b1 \<cdot> (b2 \<cdot> z))" 
+      by (metis (no_types, lifting))
+    with upred_weaken_simple[OF Sep(1) bs(2) assms(3)] Q[OF bs(3) n_incl_op_extend assms(3), of z]
+    have "pred_sem (Sep P Q) y m" unfolding pred_sem.simps by blast
+  }
+  then show ?case by (simp add: uniform_def)
+next
+  case (Wand P Q)
+  then have Q: "\<And>n m x y. \<lbrakk>(pred_sem Q) x n; n_incl m x y; m\<le>n\<rbrakk> \<Longrightarrow> (pred_sem Q) y m"
+    by (auto simp: uniform_def)
+  {
+    fix n m x y
+    assume assms: "pred_sem (Wand P Q) x n" "n_incl m x y" "m\<le>n"
+    then have I: "\<And>m b. \<lbrakk>m\<le>n; n_valid (x \<cdot> b) m; (pred_sem P) b m\<rbrakk> \<Longrightarrow> (pred_sem Q) (x \<cdot> b) m" 
+      by auto
+    {
+      fix m' z
+      assume assms2: "m'\<le>m" "n_valid (y \<cdot> z) m'" "(pred_sem P) z m'"
+      from assms(3) assms2(1) have "m'\<le>n" by linarith
+      from Q[OF I[OF this n_valid_incl_subst[OF assms(2) assms2(2,1)] assms2(3)] 
+        n_incl_extend[OF assms(2) assms2(1), of z] order.refl]
+      have "(pred_sem Q) (y \<cdot> z) m'" .
+    }
+    then have "pred_sem (Wand P Q) y m" by simp
+  }
+  then show ?case by (simp add: uniform_def)
+next
+  case (Pure b)  
+  then show ?case by (simp add: uniform_def)
+next
+  case (Persistent P)
+  {
+    fix n m x y
+    assume assms: "pred_sem (Persistent P) x n" "n_incl m x y" "m\<le>n"
+    then have I: "pred_sem P (core x) n" by simp
+    from assms(2) have "n_incl m (core x) (core y)" by (rule camera_core_mono_n)
+    with Persistent I assms(3) have "pred_sem (Persistent P) y m" 
+      unfolding pred_sem.simps uniform_def by blast
+  }
+  then show ?case by (simp add: uniform_def)
+next
+  case (Plain P)
+  then show ?case by (simp add: uniform_def)
+next
+  case (Later P)
+  then show ?case by (auto simp: uniform_def camera_n_incl_le diff_le_mono) 
+next
+  case (BUpd P)
+  then show ?case by (simp add: uniform_def n_valid_incl_subst order.trans)
+next
+  case (Impl P Q)
+  then have P: "\<And>n m x y. \<lbrakk>(pred_sem P) x n; n_incl m x y; m\<le>n\<rbrakk> \<Longrightarrow> (pred_sem P) y m"
+    by (auto simp: uniform_def)
+  from Impl(2) have Q: "\<And>n m x y. \<lbrakk>(pred_sem Q) x n; n_incl m x y; m\<le>n\<rbrakk> \<Longrightarrow> (pred_sem Q) y m"
+    by (auto simp: uniform_def)  
+  {
+    fix n m x y
+    assume assms: "pred_sem (Impl P Q) x n" "n_incl m x y" "m\<le>n"
+    then have I: "\<And>m' z. \<lbrakk>m'\<le>n;incl x z; n_valid z m'; pred_sem P z m'\<rbrakk> \<Longrightarrow> pred_sem Q z m'"
+      by auto
+    {
+      fix m' z
+      assume assms2: "m'\<le>m" "incl y z" "n_valid z m'" "pred_sem P z m'"
+      with assms(3) have "m'\<le>n" by linarith
+      from assms(2) obtain y' where y': "n_equiv m y (x\<cdot>y')" using n_incl_def by blast
+      with ofe_sym ofe_mono[OF assms2(1)] have y'_sym: "n_equiv m' (x\<cdot>y') y" by fast
+      from assms2(2) obtain z' where z': "z=y\<cdot>z'" using incl_def by blast
+      from valid_op_op_weaken[OF ofe_mono[OF assms2(1) y'] assms2(3)[simplified this]] 
+        have "n_valid ((x\<cdot>y')\<cdot>z') m'" .
+      moreover have "incl x ((x\<cdot>y')\<cdot>z')" using incl_op_extend incl_def by blast
+      moreover from P[OF assms2(4) _ order.refl, simplified z', OF total_n_incl_extend[OF y' assms2(1)]]
+        have "pred_sem P ((x\<cdot>y')\<cdot>z') m'".
+      ultimately have "pred_sem Q ((x\<cdot>y')\<cdot>z') m'" using I[OF \<open>m'\<le>n\<close>] by simp
+      from Q[OF this, of m' z, simplified z', OF total_n_incl_extend[OF y'_sym order.refl] order.refl] 
+      have "pred_sem Q z m'" unfolding z' .
+    }
+    then have "pred_sem (Impl P Q) y m" by (simp add: uniform_def)
+  }
+  then show ?case using uniform_def by blast
+next
+  case (Conj P Q)
+  then show ?case by (auto simp: uniform_def)
+next
+  case (Disj P Q)
+  then show ?case by (auto simp: uniform_def)
+next
+  case (InvP N I)
+  then show ?case unfolding pred_sem.simps uniform_def by (meson atom_sem_uniform uniform_def)
+next
+  case (Inv i)
+  then show ?case by simp
+qed
+
+definition upred_entails :: "upred \<Rightarrow> upred \<Rightarrow> bool" where
+  "upred_entails P Q \<equiv> \<forall>a n. n_valid a n \<longrightarrow> P a n \<longrightarrow> Q a n"
+definition pred_entails :: "iprop \<Rightarrow> iprop \<Rightarrow> bool" where
+  "pred_entails P Q = upred_entails (pred_sem P) (pred_sem Q)"  
+  
+definition upred_holds :: "upred \<Rightarrow> bool" where
+  "upred_holds P \<equiv> \<forall>a n. n_valid a n \<longrightarrow>  P a n"
+definition pred_holds :: "iprop \<Rightarrow> bool" where
+  "pred_holds P = upred_holds (pred_sem P)"
+end
